Progress on mailbox-sec proofs.

mailbox/verif_mailbox_bad.v
@@ -75,6 +75,7 @@ Definition last_write h := fst (find_write h (vint 0)).
 Definition comm_R bufs sh gsh g g0 g1 g2 h b := EX b1 : Z, EX b2 : Z,
   !!(-1 <= b < B /\ Forall (fun a => match a with AE v1 v2 =>
        exists r w, v1 = vint r /\ v2 = vint w /\ -1 <= r < B /\ -1 <= w < B end) h /\
+     apply_hist (vint 0) h = Some (vint b) /\
      last_two_reads (rev h) = (vint b1, vint b2) /\ repable_signed b1 /\ repable_signed b2) &&
   ghost_ref h g * ghost_var gsh (vint b1) g0 * ghost_var gsh (last_write (rev h)) g1 *
   ghost_var gsh (prev_taken (rev h)) g2 *
@@ -246,7 +247,7 @@ Definition start_write_spec :=
 Fixpoint make_shares shs lasts i : list share :=
   match lasts with
   | [] => []
-  | (g, b) :: rest => if (g || Z.eqb b i)%bool then make_shares (tl shs) rest i
+  | (g, b) :: rest => if (negb g || Z.eqb b i)%bool then make_shares (tl shs) rest i
                  else hd Share.bot shs :: make_shares (tl shs) rest i
   end.
 
@@ -257,7 +258,8 @@ Definition finish_write_spec :=
     sh1 : share, lsh : share, shs : list share, g : list val, g0 : list val, g1 : list val, g2 : list val,
     h : list hist, sh0 : share
   PRE [ ]
-   PROP (0 <= b < B; 0 <= b0 < B; Forall (fun x => 0 <= x < B) lasts; Zlength h = N; Zlength shs = N;
+   PROP (0 <= b < B; 0 <= b0 < B; Forall (fun x => 0 <= x < B) lasts; Zlength h = N;
+         Zlength lgood = N; Zlength shs = N;
          readable_share sh1; readable_share lsh; Forall readable_share shs;
          sepalg_list.list_join sh0 shs Tsh; Forall isptr comms; b <> b0; ~In b lasts; ~In b0 lasts)
    LOCAL (gvar _writing writing; gvar _last_given last_given; gvar _last_taken last_taken; gvar _comm comm)
@@ -750,6 +752,9 @@ Proof.
       apply derives_view_shift; Exists (length l) (-1) (l ++ [AE (vint v0) Empty]); unfold comm_R.
       rewrite rev_app_distr; simpl; rewrite last_two_reads_cons; simpl; cancel.
       rewrite prev_taken_cons; unfold last_write; simpl.
+      assert (apply_hist (vint 0) (l ++ [AE (vint v0) Empty]) = Some Empty).
+      { rewrite apply_hist_app; replace (apply_hist _ _) with (Some (vint v0)); simpl.
+        apply eq_dec_refl. }
       if_tac.
       + subst; simpl.
         Exists v' b0 b2; entailer!.
@@ -1040,16 +1045,6 @@ Proof.
     assert (j < i) by omega; auto.
 Qed.
 
-Lemma make_shares_out : forall b lasts shs
-  (Hb : ~In b lasts) (Hlen : Zlength lasts = Zlength shs), make_shares shs lasts b = shs.
-Proof.
-  induction lasts; auto; simpl; intros.
-  { rewrite Zlength_nil in *; destruct shs; auto; rewrite Zlength_cons, Zlength_correct in *; omega. }
-  destruct (eq_dec a b); [contradiction Hb; auto|].
-  destruct shs; rewrite !Zlength_cons in *; [rewrite Zlength_nil, Zlength_correct in *; omega|].
-  simpl; rewrite IHlasts; auto; omega.
-Qed.
-
 Lemma find_write_rest : forall d h, exists n, snd (find_write h d) = skipn n h.
 Proof.
   induction h; simpl; intros; try discriminate.
@@ -1129,34 +1124,51 @@ Proof.
   induction l1; simpl; intros.
   - rewrite sublist_same; auto.
   - rewrite Zlength_cons in *.
-    destruct shs.
+    destruct a, shs.
     { rewrite Zlength_nil, !Zlength_correct in *; omega. }
     rewrite Zlength_cons in *; simpl; rewrite IHl1; [|omega].
     rewrite sublist_S_cons with (i0 := Z.succ _); [|rewrite Zlength_correct; omega].
     unfold Z.succ; rewrite !Z.add_simpl_r.
-    destruct (eq_dec a i); auto.
+    if_tac; auto.
 Qed.
 
-Lemma make_shares_ext : forall i d l l' shs (Hlen : Zlength l = Zlength l')
+Lemma make_shares_out : forall b lgood lasts shs (Hb : ~In b lasts)
+  (Hlen1 : Zlength lgood = Zlength shs) (Hlen2 : Zlength lasts = Zlength shs),
+  make_shares shs (combine lgood lasts) b = map snd (filter fst (combine lgood shs)).
+Proof.
+  induction lgood; auto; intros.
+  destruct lasts; simpl.
+  { symmetry in Hlen2; apply Zlength_nil_inv in Hlen2; subst.
+    apply Zlength_nil_inv in Hlen1; discriminate. }
+  destruct shs; simpl.
+  { apply Zlength_nil_inv in Hlen1; discriminate. }
+  destruct (z =? b) eqn: Heq; [rewrite Z.eqb_eq in Heq; subst; contradiction Hb; simpl; auto|].
+  rewrite !Zlength_cons in *; rewrite IHlgood; try omega; simpl in *; [|tauto].
+  destruct a; auto.
+Qed.
+
+Lemma make_shares_ext : forall i d l l' lgood shs (Hlen : Zlength l = Zlength l')
   (Hi : forall j, 0 <= j < Zlength l -> Znth j l d = i <-> Znth j l' d = i),
-  make_shares shs l i = make_shares shs l' i.
+  make_shares shs (combine lgood l) i = make_shares shs (combine lgood l') i.
 Proof.
   induction l; destruct l'; simpl; intros; rewrite ?Zlength_cons, ?Zlength_nil in *; auto;
     try (rewrite Zlength_correct in *; omega).
   exploit (Hi 0); [rewrite Zlength_correct; omega|].
   rewrite !Znth_0_cons; intro Hiff.
+  destruct lgood; auto; simpl.
   rewrite (IHl l'); try omega.
-  - destruct (eq_dec a i), (eq_dec z i); tauto.
-  - intros; exploit (Hi (j + 1)); [omega|].
-    rewrite !Znth_pos_cons, !Z.add_simpl_r; auto; omega.
+  destruct (negb b); auto.
+  destruct (a =? i) eqn: Ha, (z =? i) eqn: Hz; auto; rewrite ?Z.eqb_eq, Z.eqb_neq in *; tauto.
+  { intros; exploit (Hi (j + 1)); [omega|].
+    rewrite !Znth_pos_cons, !Z.add_simpl_r; auto; omega. }
 Qed.
 
-(* The complement of make_shares. *)
-Fixpoint make_shares_inv shs (lasts : list Z) i {struct lasts} : list share :=
+(*(* The complement of make_shares. *)
+Fixpoint make_shares_inv shs lasts i {struct lasts} : list share :=
   match lasts with
   | [] => []
-  | b :: rest => if eq_dec b i then hd Share.bot shs :: make_shares_inv (tl shs) rest i
-                 else make_shares_inv (tl shs) rest i
+  | (g, b) :: rest => if (negb g || (b =? i))%bool then hd Share.bot shs :: make_shares_inv (tl shs) rest i
+                      else make_shares_inv (tl shs) rest i
   end.
 
 Lemma make_shares_minus : forall i lasts sh0 shs sh' sh1 (Hsh' : sepalg_list.list_join sh0 shs sh')
@@ -1176,44 +1188,52 @@ Proof.
     + inversion Hsh1 as [|????? Hja]; inversion Hsh' as [|????? Hjb]; subst.
       pose proof (sepalg.join_eq Hja Hjb); subst.
       eapply IHlasts; eauto; omega.
-Qed.
+Qed.*)
 
-Lemma make_shares_add : forall i i' d lasts j shs (Hj : 0 <= j < Zlength lasts)
-  (Hi : Znth j lasts d = i) (Hi' : i' <> i) (Hlen : Zlength shs >= Zlength lasts),
-  exists shs1 shs2, make_shares shs lasts i = shs1 ++ shs2 /\
-    make_shares shs (upd_Znth j lasts i') i = shs1 ++ Znth j shs Tsh :: shs2.
+Lemma make_shares_add : forall i i' d lasts lgood j shs (Hj : 0 <= j < Zlength lasts)
+  (Hi : Znth j lasts d = i) (Hgood : Znth j lgood false = true) (Hi' : i' <> i)
+  (Hlen : Zlength shs >= Zlength lasts),
+  exists shs1 shs2, make_shares shs (combine lgood lasts) i = shs1 ++ shs2 /\
+    make_shares shs (combine lgood (upd_Znth j lasts i')) i = shs1 ++ Znth j shs Tsh :: shs2.
 Proof.
   induction lasts; destruct shs; simpl; intros; rewrite ?Zlength_cons, ?Zlength_nil in *; try omega.
+  destruct lgood; [rewrite Znth_nil in Hgood; discriminate|].
   destruct (eq_dec j 0).
-  - subst; rewrite Znth_0_cons in Hi', IHlasts; rewrite !Znth_0_cons.
-    rewrite eq_dec_refl, upd_Znth0, Zlength_cons, sublist_1_cons, sublist_same; auto; try omega; simpl.
-    destruct (eq_dec i' a); [contradiction Hi'; auto|].
+  - subst; rewrite Znth_0_cons in Hi', IHlasts; rewrite !Znth_0_cons; simpl.
+    rewrite Znth_0_cons in Hgood; subst; simpl.
+    rewrite Z.eqb_refl, Zlength_cons, sublist_1_cons, sublist_same; auto; try omega; simpl.
+    rewrite <- Z.eqb_neq in Hi'; rewrite Hi'.
     eexists [], _; simpl; split; eauto.
   - rewrite Znth_pos_cons in Hi; [|omega].
+    rewrite Znth_pos_cons in Hgood; [|omega].
     rewrite Znth_pos_cons; [|omega].
-    exploit (IHlasts (j - 1) shs); try omega.
+    exploit (IHlasts lgood (j - 1) shs); auto; try omega.
     intros (shs1 & shs2 & Heq1 & Heq2).
     rewrite upd_Znth_cons; [simpl | omega].
-    exists (if eq_dec a i then shs1 else t :: shs1), shs2; rewrite Heq1, Heq2; destruct (eq_dec a i); auto.
+    exists (if (negb b || (a =? i))%bool then shs1 else t :: shs1), shs2; rewrite Heq1, Heq2;
+      if_tac; auto.
 Qed.
 
-Lemma make_shares_In : forall i lasts x shs (Hx : 0 <= x < Zlength lasts) (Hi : Znth x lasts 0 <> i)
+Lemma make_shares_In : forall i lasts lgood x shs (Hx : 0 <= x < Zlength lasts)
+  (Hi : Znth x lasts 0 <> i) (Hgood : Znth x lgood false = true)
   (Hlen : Zlength shs >= Zlength lasts),
-  In (Znth x shs Tsh) (make_shares shs lasts i).
+  In (Znth x shs Tsh) (make_shares shs (combine lgood lasts) i).
 Proof.
   induction lasts; simpl; intros.
   - rewrite Zlength_nil in *; omega.
   - destruct shs; rewrite !Zlength_cons in *; [rewrite Zlength_nil, Zlength_correct in *; omega|].
-    destruct (eq_dec x 0).
-    + subst; rewrite Znth_0_cons in Hi; rewrite Znth_0_cons.
-      destruct (eq_dec a i); [contradiction Hi | simpl]; auto.
+    destruct lgood; [rewrite Znth_nil in Hgood; discriminate|].
+    destruct (eq_dec x 0); simpl.
+    + subst; rewrite Znth_0_cons in Hi; rewrite Znth_0_cons in Hgood; rewrite Znth_0_cons.
+      rewrite <- Z.eqb_neq in Hi; rewrite Hi; subst; simpl; auto.
     + rewrite Znth_pos_cons in Hi; [|omega].
+      rewrite Znth_pos_cons in Hgood; [|omega].
       rewrite Znth_pos_cons; [|omega].
-      exploit (IHlasts (x - 1) shs); eauto; try omega.
-      destruct (eq_dec a i); simpl; auto.
+      exploit (IHlasts lgood (x - 1) shs); eauto; try omega.
+      if_tac; simpl; auto.
 Qed.
 
-Lemma make_shares_inv_In : forall i lasts x shs (Hx : 0 <= x < Zlength lasts) (Hi : Znth x lasts 0 = i)
+(*Lemma make_shares_inv_In : forall i lasts x shs (Hx : 0 <= x < Zlength lasts) (Hi : Znth x lasts 0 = i)
   (Hlen : Zlength shs >= Zlength lasts),
   In (Znth x shs Tsh) (make_shares_inv shs lasts i).
 Proof.
@@ -1227,7 +1247,7 @@ Proof.
       rewrite Znth_pos_cons; [|omega].
       exploit (IHlasts (x - 1) shs); eauto; try omega.
       destruct (eq_dec a i); simpl; auto.
-Qed.
+Qed.*)
 
 Lemma make_shares_sub : forall i lasts shs sh0 sh1 sh2 (Hlen : Zlength shs >= Zlength lasts)
   (Hsh1 : sepalg_list.list_join sh0 shs sh1) (Hsh2 : sepalg_list.list_join sh0 (make_shares shs lasts i) sh2),
@@ -1239,7 +1259,8 @@ Proof.
   - inversion Hsh1 as [|????? Hj1 Hj2]; inv Hsh2.
     destruct (sepalg_list.list_join_assoc1 Hj1 Hj2) as (? & ? & ?); eexists; eauto.
   - inversion Hsh1 as [|????? Hj1 Hj2]; subst.
-    destruct (eq_dec a i).
+    destruct a.
+    destruct (_ || _)%bool.
     + apply sepalg.join_comm in Hj1; destruct (sepalg_list.list_join_assoc1 Hj1 Hj2) as (? & ? & ?).
       exploit IHlasts; eauto; [omega|].
       intro; eapply sepalg.join_sub_trans; eauto; eexists; eauto.
@@ -1248,29 +1269,45 @@ Proof.
       eapply IHlasts; eauto; omega.
 Qed.
 
-Lemma make_shares_join : forall i d lasts shs sh0 j sh1 sh2 (Hlen : Zlength shs >= Zlength lasts)
-  (Hsh1 : sepalg_list.list_join sh0 shs sh1) (Hsh2 : sepalg_list.list_join sh0 (make_shares shs lasts i) sh2)
-  (Hin : 0 <= j < Zlength shs) (Hj : Znth j lasts d = i), exists sh', sepalg.join sh2 (Znth j shs Tsh) sh'.
+(* up *)
+Lemma combine_nil : forall {A B} (l : list A), combine l (@nil B) = [].
+Proof.
+  destruct l; auto.
+Qed.
+
+Lemma make_shares_join : forall i d lasts lgood shs sh0 j sh1 sh2
+  (Hlen : Zlength shs >= Zlength lasts)
+  (Hsh1 : sepalg_list.list_join sh0 shs sh1)
+  (Hsh2 : sepalg_list.list_join sh0 (make_shares shs (combine lgood lasts) i) sh2)
+  (Hin : 0 <= j < Zlength shs) (Hj : Znth j lasts d = i),
+  exists sh', sepalg.join sh2 (Znth j shs Tsh) sh'.
 Proof.
   induction lasts; destruct shs; simpl; intros; rewrite ?Zlength_nil, ?Zlength_cons in *;
     try (rewrite Zlength_correct in *; omega); try omega.
-  { rewrite Znth_overflow in Hj; [|rewrite Zlength_nil; omega].
-    inv Hsh2.
+  { rewrite Znth_nil in Hj.
+    rewrite combine_nil in Hsh2; inv Hsh2.
     exploit (Znth_In j (t :: shs) Tsh); [rewrite Zlength_cons; auto|].
     intro Hin'; apply in_split in Hin'.
     destruct Hin' as (? & ? & Heq); rewrite Heq in Hsh1.
     apply list_join_comm in Hsh1; inv Hsh1; eauto. }
   destruct (eq_dec j 0).
   - subst j; rewrite Znth_0_cons in Hj; rewrite Znth_0_cons; subst.
-    rewrite eq_dec_refl in Hsh2.
+    destruct lgood; simpl in Hsh2; [inv Hsh2; inv Hsh1; eauto|].
+    rewrite Z.eqb_refl in Hsh2.
     inversion Hsh1 as [|????? Hj1 Hj2]; subst.
     apply sepalg.join_comm in Hj1; destruct (sepalg_list.list_join_assoc1 Hj1 Hj2) as (? & ? & ?).
-    exploit make_shares_sub; eauto; [omega|].
+    exploit (make_shares_sub i (combine lgood lasts)); eauto.
+    { rewrite Zlength_combine, Z.ge_le_iff, Z.min_le_iff; omega. }
+    { destruct b; eauto. }
     intro; eapply sepalg.join_sub_joins_trans; eauto.
   - rewrite Znth_pos_cons in Hj; [|omega].
     rewrite Znth_pos_cons; [|omega].
-    inversion Hsh1 as [|????? Hj1 Hj2].
-    destruct (eq_dec a i); subst.
+    inversion Hsh1 as [|????? Hj1 Hj2]; subst.
+    destruct lgood; simpl in Hsh2.
+    { inv Hsh2.
+      apply sepalg.join_comm in Hj1; destruct (sepalg_list.list_join_assoc1 Hj1 Hj2) as (? & ? & ?).
+      eapply (IHlasts []); eauto; try constructor; omega. }
+    destruct (_ || _)%bool.
     + apply sepalg.join_comm in Hj1; destruct (sepalg_list.list_join_assoc1 Hj1 Hj2) as (? & ? & ?).
       eapply IHlasts; eauto; omega.
     + inversion Hsh2 as [|????? Hj1']; subst.
@@ -1282,19 +1319,19 @@ Lemma data_at_buffer_cohere : forall sh1 sh2 v1 v2 p, readable_share sh1 ->
   data_at sh1 tbuffer v1 p * data_at sh2 tbuffer v2 p |--
   data_at sh1 tbuffer v1 p * data_at sh2 tbuffer v1 p.
 Proof.
-  intros; unfold data_at, field_at, at_offset; Intros.
-  apply andp_right; [apply prop_right; auto|].
-  rewrite !data_at_rec_eq; unfold withspacer, at_offset; simpl.
-  rewrite !data_at_rec_eq; simpl.
-  apply mapsto_value_cohere; auto.
+  intros.
+  repeat unfold_data_at 1%nat.
+  rewrite !field_at_data_at'; simpl; entailer.
+  apply data_at_value_cohere; auto.
 Qed.
 
-(* The relationship between the last_taken array and the shares held by the writer is
+(*(* The relationship between the last_taken array and the shares held by the writer is
    preserved by the action of the loop body. *)
-Lemma upd_write_shares : forall bufs b b0 lasts shs sh0 (Hb : 0 <= b < B) (Hb0 : 0 <= b0 < B)
+Lemma upd_write_shares : forall bufs b b0 lgood lasts shs sh0 (Hb : 0 <= b < B) (Hb0 : 0 <= b0 < B)
   (Hlasts : Forall (fun x : Z => 0 <= x < B) lasts) (Hshs : Zlength shs = N)
   (Hread : Forall readable_share shs) (Hsh0 : sepalg_list.list_join sh0 shs Tsh)
   (Hdiff : b <> b0) (Hout : ~ In b lasts) (Hout0 : ~ In b0 lasts) (Hlasts : Zlength lasts = N)
+  (Hlgood : Zlength lgood = N)
   bsh' v' (Hv' : -1 <= v' < B) h' (Hh' : 0 <= Zlength h' < N)
   (Hbsh' : sepalg_list.list_join sh0 (sublist (Zlength h' + 1) N shs) bsh')
   bsh (Hbsh : sepalg.join bsh' (Znth (Zlength h') shs Tsh) bsh),
@@ -1528,7 +1565,7 @@ Proof.
         split; intro; subst; tauto.
       * rewrite Znth_overflow, Znth_overflow with (al := h' ++ [vint v']); auto; [reflexivity|].
         rewrite Zlength_app, Zlength_cons, Zlength_nil; omega.
-Qed.
+Qed.*)
 
 Lemma body_finish_write : semax_body Vprog Gprog f_finish_write finish_write_spec.
 Proof.
@@ -1538,14 +1575,18 @@ Proof.
   forward.
   assert_PROP (Zlength (map (fun i => vint i) lasts) = N) by entailer!.
   rewrite Zlength_map in *.
+  assert (Zlength (combine lgood lasts) = N).
+  { rewrite Zlength_combine, Z.min_l; omega. }
+  assert (Zlength (combine lgood shs) = N).
+  { rewrite Zlength_combine, Z.min_l; omega. }
   rewrite <- seq_assoc.
   forward_for_simple_bound N (EX i : Z, PROP ( )
    LOCAL (temp _w (vint b); temp _last (vint b0); gvar _writing writing; gvar _last_given last_given;
-          gvar _last_taken last_taken; gvar _comm comm; gvar _lock lock)
+          gvar _last_taken last_taken; gvar _comm comm)
    SEP (data_at Ews tint (vint b) writing; data_at Ews tint (vint b0) last_given;
-        data_at sh1 (tarray (tptr tint) N) comms comm; data_at sh1 (tarray (tptr tlock) N) locks lock;
+        data_at sh1 (tarray (tptr tint) N) comms comm;
         EX t' : list nat, EX h' : list val, !!(Zlength t' = i /\ Zlength h' = i) &&
-          fold_right sepcon emp (map (fun r => comm_loc lsh (Znth r locks Vundef) (Znth r comms Vundef)
+          fold_right sepcon emp (map (fun r => comm_loc (Znth r lgood false) lsh (Znth r comms Vundef)
             (Znth r g Vundef) (Znth r g0 Vundef) (Znth r g1 Vundef) (Znth r g2 Vundef) bufs (Znth r shs Tsh)
             gsh2 (Znth r h [] ++ if zlt r i then [(Znth r t' O, AE (Znth r h' Vundef) (vint b))] else []))
             (upto (Z.to_nat N))) *
@@ -1557,9 +1598,9 @@ Proof.
             fold_right sepcon emp (map (fun r =>
               ghost_var gsh1 (vint (Znth r lasts' (-1))) (Znth r g2 Vundef)) (upto (Z.to_nat N))) *
             fold_right sepcon emp (map (fun a => EX sh : share,
-              !!(if eq_dec a b0 then sepalg_list.list_join sh0 (make_shares shs (sublist 0 i lasts') a) sh
-                 else if eq_dec a b then sepalg_list.list_join sh0 (sublist i N shs) sh
-                 else sepalg_list.list_join sh0 (make_shares shs lasts' a) sh) &&
+              !!(if eq_dec a b0 then sepalg_list.list_join sh0 (make_shares shs (combine lgood (sublist 0 i lasts')) a) sh
+                 else if eq_dec a b then sepalg_list.list_join sh0 (map snd (filter fst (sublist i N (combine lgood shs)))) sh
+                 else sepalg_list.list_join sh0 (make_shares shs (combine lgood lasts') a) sh) &&
               EX v : Z, @data_at CompSpecs sh tbuffer (vint v) (Znth a bufs Vundef)) (upto (Z.to_nat B))))).
   { unfold N; computable. }
   { unfold N; computable. }
@@ -1574,11 +1615,11 @@ Proof.
       destruct (zlt a 0); [omega | rewrite app_nil_r; auto]. }
     apply map_ext; intro.
     f_equal; extensionality; f_equal; f_equal.
+    rewrite sublist_nil, combine_nil; simpl.
     apply prop_ext.
     destruct (eq_dec a b0); [|destruct (eq_dec a b); [|reflexivity]].
     - split; intro Hx; [subst; constructor | inv Hx; auto].
-    - subst; rewrite sublist_same, make_shares_out; auto; try reflexivity.
-      replace (Zlength lasts) with N; auto.
+    - subst; rewrite sublist_same, make_shares_out; unfold share in *; auto; try reflexivity; omega.
     - rewrite (list_Znth_eq 0 lasts) at 1.
       replace (length lasts) with (Z.to_nat N).
       apply map_ext.
@@ -1591,146 +1632,164 @@ Proof.
       apply Forall_Znth.
       { rewrite Hcomms; auto. }
       apply Forall_impl with (P := isptr); auto. }
-    rewrite <- lock_struct_array.
     rewrite (extract_nth_sepcon (map _ (upto (Z.to_nat N))) i);
       [|rewrite Zlength_map; auto].
-    rewrite Znth_map with (d' := N); [|rewrite Zlength_upto; auto].
-    rewrite Znth_upto; [|rewrite Z2Nat.id; auto; omega].
+    erewrite Znth_map, Znth_upto by (rewrite ?Zlength_upto, Z2Nat.id; auto; omega).
     destruct (zlt i i); [omega | rewrite app_nil_r].
-    rewrite comm_loc_isptr; Intros.
-    forward.
-    rewrite (extract_nth_sepcon (map _ (upto (Z.to_nat B))) b); [|rewrite Zlength_map, Zlength_upto; auto].
-    rewrite Znth_map with (d' := B), Znth_upto; rewrite ?Zlength_upto, ?Z2Nat.id; auto; try omega.
+    rewrite (extract_nth_sepcon (map _ (upto (Z.to_nat B))) b) by (rewrite Zlength_map, Zlength_upto; auto).
+    erewrite Znth_map, Znth_upto by (rewrite ?Zlength_upto, ?Z2Nat.id; auto; omega).
     Intros bsh.
-    destruct (eq_dec b b0); [absurd (b = b0); auto|].
+    destruct (eq_dec b b0); [contradiction|].
     match goal with H : if eq_dec b b then _ else _ |- _ => rewrite eq_dec_refl in H end.
-    match goal with H : sepalg_list.list_join _ (sublist i N shs) _ |- _ =>
-      rewrite sublist_split with (mid := i + 1) in H; try omega;
-      apply list_join_comm, sepalg_list.list_join_unapp in H; destruct H as (bsh' & ? & Hsh) end.
-    rewrite sublist_len_1 with (d := Tsh), <- sepalg_list.list_join_1 in Hsh; [|omega].
+    match goal with H : sepalg_list.list_join _ (map _ _) _ |- _ =>
+      rewrite sublist_split with (mid := i + 1), sublist_len_1 with (d := (false, Tsh)), filter_app,
+        map_app, Znth_combine in H by omega; simpl in H;
+        apply list_join_comm, sepalg_list.list_join_unapp in H;
+        destruct H as (shi & Hshi & Hbsh) end.
     rewrite (extract_nth_sepcon (map _ (upto (Z.to_nat N))) i); [|rewrite Zlength_map; auto].
     rewrite (extract_nth_sepcon (map _ (upto (Z.to_nat N))) i); [|rewrite Zlength_map; auto].
     erewrite !Znth_map; rewrite ?Znth_upto; rewrite ?Znth_upto, ?Zlength_upto; rewrite ?Z2Nat.id; auto; try omega.
-    rewrite Znth_overflow with (al := h'); [|omega].
+    rewrite Znth_overflow with (al := h'); [simpl | omega].
     destruct (zlt i i); [clear - l; omega|].
-    forward_call (lsh, Znth i comms Vundef, Znth i g Vundef, Znth i locks Vundef, vint 0, vint b, Znth i h [],
-      fun (h : hist) (v : val) => !!(v = vint b) &&
-        ghost_var gsh1 (vint b0) (Znth i g1 Vundef) *
-        ghost_var gsh1 (vint (Znth i lasts 0)) (Znth i g2 Vundef) *
-        EX v : Z, data_at (Znth i shs Tsh) tbuffer (vint v) (Znth b bufs Vundef),
-      comm_R bufs (Znth i shs Tsh) gsh2 (Znth i g0 Vundef) (Znth i g1 Vundef) (Znth i g2 Vundef),
-        fun (h : hist) (v : val) => EX b' : Z, !!(v = vint b' /\ -1 <= b' < B) &&
-          ghost_var gsh1 (vint b) (Znth i g1 Vundef) *
-          ghost_var gsh1 (vint (if eq_dec b' (-1) then b0 else Znth i lasts 0)) (Znth i g2 Vundef) *
-          if eq_dec b' (-1) then EX v : Z, data_at (Znth i shs Tsh) tbuffer (vint v) (Znth (Znth i lasts 0) bufs Vundef)
-          else !!(b' = b0) && EX v' : Z, data_at (Znth i shs Tsh) tbuffer (vint v') (Znth b0 bufs Vundef)).
-    { rewrite <- !sepcon_assoc; rewrite (sepcon_comm _ (EX v : Z, @data_at CompSpecs bsh tbuffer (vint v) _)).
-      rewrite !sepcon_assoc; eapply derives_trans; [apply sepcon_derives; [|apply derives_refl]|].
-      { instantiate (1 := (EX v : Z, data_at bsh' tbuffer (vint v) (Znth b bufs Vundef)) *
-          (EX v : Z, data_at (Znth i shs Tsh) tbuffer (vint v) (Znth b bufs Vundef))).
-        Intro v0; Exists v0 v0; rewrite (data_at_share_join _ _ _ _ _ _ Hsh); auto. }
-      fast_cancel. }
-    { repeat (split; auto).
-      unfold AE_spec; intros.
-      intros ??????? Ha.
-      unfold comm_R; unfold comm_R at 1 in Ha.
-      rewrite rev_app_distr in Ha; simpl in Ha.
-      rewrite last_two_reads_cons, prev_taken_cons in Ha.
-      rewrite flatten_sepcon_in_SEP.
-      rewrite extract_exists_in_SEP; Intro b'.
-      rewrite extract_exists_in_SEP; Intro b1.
-      rewrite extract_exists_in_SEP; Intro b2.
-      rewrite <- flatten_sepcon_in_SEP.
-      rewrite !sepcon_andp_prop', !sepcon_andp_prop.
-      erewrite extract_prop_in_SEP with (n := O); simpl; eauto.
-      erewrite extract_prop_in_SEP with (n := O); simpl; eauto.
-      Intros.
-      assert (repable_signed b) by (apply repable_buf; omega).
-      destruct (eq_dec vc Empty).
-      { subst; assert (b = -1) by (apply Empty_inj; auto); omega. }
-      apply semax_pre with (P' := PROPx P (LOCALx Q (SEPx (
-        (ghost_var gsh1 (vint b0) (Znth i g1 Vundef) *
-         ghost_var gsh2 (last_write (rev hx)) (Znth i g1 Vundef)) ::
-        (ghost_var gsh1 (vint (Znth i lasts 0)) (Znth i g2 Vundef) *
-         ghost_var gsh2 (prev_taken (rev hx)) (Znth i g2 Vundef)) ::
-        (ghost_var gsh2 (vint b1) (Znth i g0 Vundef) *
-         (if eq_dec b' (-1) then EX v1 : Z, @data_at CompSpecs (Znth i shs Tsh) tbuffer (vint v1) (Znth b2 bufs Vundef)
-          else EX v1 : Z, @data_at CompSpecs (Znth i shs Tsh) tbuffer (vint v1) (Znth b' bufs Vundef)) *
-         (EX v1 : Z, @data_at CompSpecs (Znth i shs Tsh) tbuffer (vint v1) (Znth b bufs Vundef))) :: R)))).
-      { go_lowerx; cancel. }
-      assert_PROP (last_write (rev hx) = vint b0) as Hwrite.
-      { go_lowerx; apply sepcon_derives_prop.
-        rewrite sepcon_comm; apply ghost_var_inj; auto. }
-      assert_PROP (prev_taken (rev hx) = vint (Znth i lasts 0)) as Hprev.
-      { go_lowerx.
-        rewrite <- sepcon_assoc, (sepcon_comm (_ * _) (_ * ghost_var _ _ _)).
-        do 2 apply sepcon_derives_prop.
-        rewrite sepcon_comm; apply ghost_var_inj; auto. }
-      rewrite <- Hprev, <- Hwrite in *.
-      erewrite !ghost_var_share_join; eauto.
-      apply ghost_var_update with (v' := vint b).
-      rewrite <- flatten_sepcon_in_SEP, sepcon_comm, flatten_sepcon_in_SEP.
-      apply ghost_var_update with (v' := if eq_dec b' (-1) then last_write (rev hx) else prev_taken (rev hx)).
-      rewrite <- !(ghost_var_share_join _ _ _ _ _ gsh1_gsh2_join).
-      eapply semax_pre, Ha.
-      go_lowerx.
-      rewrite (sepcon_comm _ (weak_precise_mpred _ && _)).
-      rewrite <- emp_sepcon at 1; rewrite !sepcon_assoc; apply sepcon_derives.
-      { apply andp_right; auto; eapply derives_trans; [|apply comm_R_precise]; auto. }
-      Exists b b1 b2.
-      rewrite !sepcon_andp_prop'.
-      apply andp_right.
-      { apply prop_right; repeat (split; [solve [auto; omega]|]).
-      rewrite Forall_app; split; [split; [|constructor]; auto | auto].
-      subst; repeat eexists; auto; omega. }
-      destruct (eq_dec b (-1)); [omega|].
-      rewrite (sepcon_comm (_ * _)); Exists b'.
-      rewrite !sepcon_andp_prop'; apply andp_right; [apply prop_right; auto|].
-      assert (last_two_reads (rev hx) = (vint b1, vint b2)) as Hlast by assumption.
-      erewrite take_read, Hlast in *; try (rewrite rev_involutive; eauto).
-      unfold last_write in *; simpl in *.
-      destruct (eq_dec vc Empty); [absurd (vc = Empty); auto|].
-      assert (Znth i lasts 0 = if eq_dec vx Empty then b2 else b1).
-      { assert (repable_signed (Znth i lasts 0)).
-        { apply Forall_Znth; [omega|].
-          eapply Forall_impl; [|eauto]; intros.
-          apply repable_buf; simpl in *; omega. }
-        destruct (eq_dec vx Empty); apply repr_inj_signed; auto; congruence. }
-      destruct (eq_dec vx Empty); subst; fast_cancel.
-      + assert (b' = -1) by (apply Empty_inj; auto; apply repable_buf; auto).
-        subst; rewrite !eq_dec_refl.
-        rewrite Hwrite; simpl; cancel.
-        exploit find_write_read.
-        { rewrite rev_involutive; eauto. }
+    set (gi := Znth i g Vundef).
+    set (g0i := Znth i g0 Vundef).
+    set (g1i := Znth i g1 Vundef).
+    set (g2i := Znth i g2 Vundef).
+    set (c := Znth i comms Vundef).
+    set (sh := Znth i shs Tsh) in *.
+    set (hi := Znth i h []).
+    set (good := Znth i lgood false) in *.
+    Intro vb.
+    forward_call (c, b,
+      (if good then data_at sh tbuffer (vint vb) (Znth b bufs Vundef) else emp) *
+      ghost_var gsh1 (vint b0) g1i * ghost_var gsh1 (vint (Znth i lasts 0)) g2i * ghost_hist lsh hi gi,
+      fun _ : Z => comm_inv good c bufs sh gi g0i g1i g2i gsh2, [0],
+      fun shw v => !!(shw = Tsh) &&
+       (if good then (EX h : list AE_hist_el, comm_R bufs sh gsh2 gi g0i g1i g2i h v) *
+        data_at sh tbuffer (vint vb) (Znth b bufs Vundef)
+        else (EX h : list AE_hist_el, ghost_ref h gi) * (EX v0 : val, ghost_var gsh2 v0 g0i) *
+          (EX v0 : val, ghost_var gsh2 v0 g1i) * (EX v0 : val, ghost_var gsh2 v0 g2i) *
+          fold_right sepcon emp (map (data_at_ sh tbuffer) bufs)) *
+        ghost_var gsh1 (vint b0) g1i * ghost_var gsh1 (vint (Znth i lasts 0)) g2i * ghost_hist lsh hi gi,
+      fun b' => !!(good = true -> b' = -1 \/ b' = b0) &&
+        (if good then EX v : Z, data_at sh tbuffer (vint v)
+          (Znth (if eq_dec b' (-1) then Znth i lasts 0 else b0) bufs Vundef) else emp) *
+        ghost_var gsh1 (vint b) g1i *
+        ghost_var gsh1 (vint (if eq_dec b' (-1) then b0 else Znth i lasts 0)) g2i *
+        EX t : _, !!(newer hi t) && ghost_hist lsh (hi ++ [(t, AE (vint b') (vint b))]) gi).
+    { unfold comm_loc at 1; simpl; cancel.
+      destruct good; simpl in *.
+      + rewrite <- sepalg_list.list_join_1 in Hbsh.
+        rewrite <- (data_at_share_join _ _ _ _ _ _ Hbsh); cancel.
+      + inv Hbsh; subst Frame; simpl; cancel. }
+    { lapply (repable_buf b); [|omega].
+      split; auto; split.
+      { apply derives_view_shift.
+        unfold comm_inv; simpl.
+        Intro v; Exists Tsh v; entailer!.
+        if_tac; cancel.
+        rewrite <- exp_sepcon1; auto. }
+      intros.
+      assert (lsh <> Share.bot) by (intro; subst; contradiction unreadable_bot).
+      view_shift_intros; subst sh2; if_tac; unfold comm_inv; simpl.
+      + view_shift_intro l.
+        unfold comm_R at 1.
+        view_shift_intro b1; view_shift_intro b2; view_shift_intro v'; view_shift_intros.
+        rewrite <- !sepcon_assoc, (sepcon_comm _ (ghost_ref _ _)).
+        rewrite (sepcon_comm _ (ghost_hist _ _ _)).
+        rewrite <- !sepcon_assoc, 7sepcon_assoc.
+        apply view_shift_assert with (PP := hist_incl hi l).
+        { apply sepcon_derives_prop, hist_ref_incl; auto. }
+        intros ?%hist_incl_lt.
+        etransitivity; [apply view_shift_sepcon1, hist_add'; auto|].
+        rewrite <- !sepcon_assoc, (sepcon_comm _ (ghost_var gsh2 _ g1i)).
+        rewrite <- !sepcon_assoc, (sepcon_comm _ (ghost_var gsh1 _ g1i)).
+        erewrite <- !sepcon_assoc, ghost_var_share_join' by eauto.
+        view_shift_intros.
+        rewrite !sepcon_assoc; etransitivity; [apply view_shift_sepcon1,
+          ghost_var_update with (v' := vint b)|].
+        erewrite <- ghost_var_share_join by eauto.
+        rewrite <- !sepcon_assoc, (sepcon_comm _ (ghost_var gsh2 _ g2i)).
+        rewrite <- !sepcon_assoc, (sepcon_comm _ (ghost_var gsh1 _ g2i)).
+        erewrite <- !sepcon_assoc, ghost_var_share_join' by eauto.
+        view_shift_intros.
+        rewrite !sepcon_assoc; etransitivity; [apply view_shift_sepcon1,
+          ghost_var_update with (v' := vint (if eq_dec v0 (-1) then b0 else Znth i lasts 0))|].
+        erewrite <- ghost_var_share_join by eauto.
+        apply derives_view_shift; Exists (length l) b (l ++ [AE (vint v0) (vint b)]); unfold comm_R.
+        rewrite !rev_app_distr; unfold last_write in *; simpl;
+          rewrite last_two_reads_cons, prev_taken_cons.
+        destruct (eq_dec (vint b) Empty).
+        { apply Empty_inj in e; auto; subst; omega. }
+        destruct (eq_dec b (-1)); [omega|].
+        assert (Forall (fun a => match a with AE v1 v2 => exists r w,
+          v1 = vint r /\ v2 = vint w /\ -1 <= r < B /\ -1 <= w < B end)
+          (l ++ [AE (vint v0) (vint b)])).
+        { rewrite Forall_app; repeat constructor; auto.
+          exists v0, b; repeat (split; auto; try omega). }
+        assert (apply_hist (vint 0) (l ++ [AE (vint v0) (vint b)]) = Some (vint b)).
+        { rewrite apply_hist_app; replace (apply_hist _ _) with (Some (vint v0)); simpl.
+          apply eq_dec_refl. }
+        match goal with H : _ = prev_taken _ |- _ =>
+          erewrite take_read in H by (rewrite rev_involutive; eauto) end.
+        match goal with H : last_two_reads _ = _ |- _ => rewrite H in * end.
+        if_tac; Intro v; Exists v b1 b2 vb.
+        * subst; match goal with H : vint _ = _ |- _ => rewrite eq_dec_refl in H end.
+          exploit (repr_inj_signed b2 (Znth (Zlength t') lasts 0)); auto.
+          { apply Forall_Znth; [omega|].
+            eapply Forall_impl; [|eauto]; simpl; intros; apply repable_buf; omega. }
+          { simpl in *; congruence. }
+          intro; entailer!.
+          erewrite find_write_read by (rewrite ?rev_involutive; eauto; discriminate).
+          replace (fst _) with (vint b0).
+          rewrite (sepcon_comm _ (ghost_ref _ _)); cancel.
+        * destruct (eq_dec (vint v0) Empty); [apply Empty_inj in e; auto; contradiction|].
+          exploit (write_val (rev l)); [rewrite rev_involutive; eauto|].
+          intros [|]; [contradiction|].
+          exploit (repr_inj_signed v0 b0); auto.
+          { apply repable_buf; omega. }
+          { congruence. }
+          exploit (repr_inj_signed (Znth i lasts 0) b1); auto.
+          { apply Forall_Znth; [omega|].
+            eapply Forall_impl; [|eauto]; simpl; intros; apply repable_buf; omega. }
+          { simpl in *; congruence. }
+          intros; entailer!.
+          rewrite sepcon_comm; apply derives_refl'; f_equal; f_equal.
+          unfold last_two_reads in *.
+          destruct (find_read _ _); match goal with H : (_, _) = (_, _) |- _ => inv H; auto end.
+      + view_shift_intro l.
+        rewrite <- !sepcon_assoc, (sepcon_comm _ (ghost_ref _ _)).
+        rewrite (sepcon_comm _ (ghost_hist _ _ _)).
+        rewrite <- !sepcon_assoc, 6sepcon_assoc.
+        apply view_shift_assert with (PP := hist_incl hi l).
+        { apply sepcon_derives_prop, hist_ref_incl; auto. }
+        intros ?%hist_incl_lt.
+        etransitivity; [apply view_shift_sepcon1, hist_add'; auto|].
+        view_shift_intro b0'; view_shift_intro b1'; view_shift_intro b2'.
+        rewrite <- !sepcon_assoc, (sepcon_comm _ (ghost_var gsh2 _ g1i)).
+        rewrite <- !sepcon_assoc, (sepcon_comm _ (ghost_var gsh1 _ g1i)).
+        erewrite <- !sepcon_assoc, ghost_var_share_join' by eauto.
+        view_shift_intros.
+        rewrite !sepcon_assoc; etransitivity; [apply view_shift_sepcon1,
+          ghost_var_update with (v' := vint b)|].
+        erewrite <- ghost_var_share_join by eauto.
+        rewrite <- !sepcon_assoc, (sepcon_comm _ (ghost_var gsh2 _ g2i)).
+        rewrite <- !sepcon_assoc, (sepcon_comm _ (ghost_var gsh1 _ g2i)).
+        erewrite <- !sepcon_assoc, ghost_var_share_join' by eauto.
+        view_shift_intros.
+        rewrite !sepcon_assoc; etransitivity; [apply view_shift_sepcon1,
+          ghost_var_update with (v' := vint (if eq_dec v0 (-1) then b0 else Znth i lasts 0))|].
+        erewrite <- ghost_var_share_join by eauto.
+        apply derives_view_shift.
+        Exists (length l) b (l ++ [AE (vint v0) (vint b)])
+          (vint (if eq_dec v0 (-1) then b0 else Znth i lasts 0)) (vint b) b0'; entailer!.
         { discriminate. }
-        intros ->; rewrite Hwrite; auto.
-      + assert (exists rest, find_write (rev hx) (vint 0) = (vint b', rest)) as (? & Hwrite').
-        { replace hx with (rev (rev hx)) in Hvx by (apply rev_involutive).
-          destruct (rev hx); simpl in *.
-          { assert (b' = 0); [|subst; eauto].
-            apply repr_inj_signed.
-            * apply repable_buf; auto.
-            * split; computable.
-            * congruence. }
-          destruct a.
-          rewrite apply_hist_app in Hvx.
-          destruct (apply_hist (vint 0) (rev l)); [simpl in * | discriminate].
-          destruct (eq_dec r v); [|discriminate].
-          inv Hvx.
-          destruct (eq_dec (vint b') Empty); [absurd (vint b' = Empty); auto | eauto]. }
-        rewrite Hwrite' in Hwrite.
-        assert (b' = b0).
-        { apply repr_inj_signed; [apply repable_buf | apply repable_buf | simpl in *; congruence]; auto; omega. }
-        subst.
-        destruct (eq_dec b0 (-1)); [subst; contradiction n3; auto|].
-        rewrite !sepcon_andp_prop', !sepcon_andp_prop; apply andp_right; [apply prop_right; auto|].
-        unfold last_two_reads in Hlast; destruct (find_read (rev hx) (vint 1)); inv Hlast.
-        simpl; cancel. }
-    Intros x b'; destruct x as (t, v); simpl in *.
-    gather_SEP 0 9; replace_SEP 0 (fold_right sepcon emp (map (fun r =>
-      comm_loc lsh (Znth r locks Vundef) (Znth r comms Vundef) (Znth r g Vundef) (Znth r g0 Vundef)
+        rewrite sepcon_comm; auto. }
+    Intros b' t.
+    gather_SEP 0 4 8; replace_SEP 0 (fold_right sepcon emp (map (fun r =>
+      comm_loc (Znth r lgood false) lsh (Znth r comms Vundef) (Znth r g Vundef) (Znth r g0 Vundef)
         (Znth r g1 Vundef) (Znth r g2 Vundef) bufs (Znth r shs Tsh) gsh2 (Znth r h [] ++
-        (if zlt r (i + 1) then [(Znth r (t' ++ [t]) 0%nat, AE (Znth r (h' ++ [v]) Vundef) (vint b))] else [])))
+        (if zlt r (i + 1) then [(Znth r (t' ++ [t]) 0%nat, AE (Znth r (h' ++ [vint b']) Vundef) (vint b))] else [])))
       (upto (Z.to_nat N)))).
     { go_lower.
       rewrite replace_nth_sepcon; apply sepcon_list_derives; rewrite upd_Znth_Zlength;
