progs/verif_example.v
@@ -100,20 +100,6 @@ Proof.
   (* temporarily broken *)
 Admitted.
 
-(* up *)
-Lemma field_at_data_at' : forall sh t gfs v p, field_at sh t gfs v p =
-  !!field_compatible t gfs p &&
-  data_at sh (nested_field_type t gfs) v (offset_val (nested_field_offset t gfs) p).
-Proof.
-  intros.
-  rewrite field_at_data_at.
-  unfold field_address.
-  if_tac.
-  - rewrite prop_true_andp; auto.
-  - rewrite prop_false_andp by auto.
-    rewrite data_at_isptr, prop_false_andp; auto.
-Qed.
-
 Lemma sum_base : forall l i, fold_right Z.add i l = fold_right Z.add 0 l + i.
 Proof.
   induction l; auto; simpl; intro.
